src/hint.mli
@@ -10,4 +10,5 @@ val lookup_tbl : string -> hint_db
 val apply_hints : Ltac_plugin.Tacinterp.value -> hint_db -> unit Proofview.tactic
 
 val pretty_hints : (Constr.t -> string) -> hint_db -> string
+val gather_hints : hint_db -> Constr.t list
 
